
---
title: 若干极限问题
tag: [](/math/index.md)
---

<style>
.frame {
    border: 1px solid;
    border-radius: 0.2em;
    padding: 0.5em;
    margin: 0;
    margin-bottom: 1em;
}
.frame>a {
    padding: 0;
}
</style>

<script>
document.addEventListener('DOMContentLoaded', function() {
    const blocks = document.querySelectorAll('.frame');
    
    blocks.forEach((block, index) => {
        const counter = document.createElement('a');
        const counterNumber = (index + 1).toString().padStart(4, '0');
        
        counter.textContent = counterNumber;
        counter.href = `#block-${counterNumber}`;
        
        counter.style.display = 'block';
        counter.style.textAlign = 'right';
        counter.style.padding = '2px 6px';
        counter.style.fontFamily = 'monospace';
        counter.style.fontSize = '12px';
        counter.style.textDecoration = 'none';
        
        block.insertAdjacentElement('beforebegin', counter);
        
        block.id = `block-${counterNumber}`;
    });
});
</script>

$\gdef\spaces#1{~ #1 ~}$

<div class="frame">

$$
\lim_{x \to \infty} ~ x^2 \ln(1+\tfrac1x) - x
\spaces\iff 
\lim_{x \to 0} ~ \frac1{x^2} \ln(1+x) - \frac1{x}
$$

我们直接使用 $\ln(1+x) \sim x-\frac{x^2}2$, 从而得到 $\lim\square = -\frac12$. 也就是说

$$
\lim_{x \to \infty} \frac{(1+\frac1x)^{x^2}}{e^x} 
\spaces= \lim_{x \to \infty} \frac{e^{x^2\ln(1+\frac1x)}}{e^x}
\spaces= \lim_{x \to \infty} e^{x^2\ln(1+\frac1x) - x}
\spaces= e^{-\frac12}
$$

</div>


<div class="frame">

$$
\begin{aligned}
\lim_{x \to \infty} \bigg(\frac{x^2}{(x-a)(x+b)}\bigg)^x
\spaces&= \lim_{x \to \infty} \Big(\frac{x}{x-a}\Big)^x \cdot \Big(\frac{x}{x+b}\Big)^x \\
\spaces&= \lim_{x \to \infty} \Big(1-\frac{a}{x}\Big)^{-x} \cdot \Big(1+\frac{b}{x}\Big)^{-x} \\
\spaces&= e^{a-b}
\end{aligned}
$$

</div>

<div class="frame">

$$
\lim\limits_{x \to 0} \frac{\sqrt{1+\sin x}-\sqrt{1-\sin x}}{x}
$$

$\sin x \sim x - \frac{x^3}6$, $(1+x)^{\frac12} \sim 1+\frac{x}2 - \frac{x^3}{12}$, $(1-x)^{\frac12} \sim 1-\frac{x}2+\frac{x^3}{12}$. 分子 $\sim x - \frac{x^3}{6}$. $\lim \square = 1$. 

</div>

<div class="frame">

$$
\lim\limits_{x \to 0} \Big(\frac{e^x + e^{-x}}{2}\Big)^{\frac1{x^2}}
$$

取对数, $\lim\limits_{x \to 0} \exp(\frac1{x^2}\ln(\frac{e^x + e^{-x}}{2})) \sim \lim\limits_{x \to 0} \exp(\frac1{x^2}\ln(1+\frac{x^2}2)) \sim \lim\limits_{x \to 0} \exp(\frac1{x^2} \cdot \frac{x^2}2) = e^{\frac12}$. 

</div>

<div class="frame">

$$ \lim\limits_{x \to 0} \frac{\ln(1+x) - x\cos x}{x^2} $$

$\cos x \sim 1 - \frac{x^2}2 + \frac{x^4}{24} + \Re\sum_{n \geqslant 5} i^n\frac{x^n}{n!}$. $\square \sim \frac{x - \frac{x^2}2 + \frac{x^3}3 - x + \frac{x^3}2}{x^2} = \frac{-\frac{x^2}2+\frac{5x^3}{6}}{x^2} = -\frac{1}{2}$.

</div>

<div class="frame">

$$ \lim\limits_{x \to 0} \frac{e^x\sin x - x(1+x)}{x^3} $$


$\square \sim \frac{(1+x+\frac{x^2}{2}+\frac{x^3}{6})(x - \frac{x^3}6) - x - x^2}{x^3} \sim \frac{\frac{x^3}2 - \frac{x^3}6}{x^3} = \frac{1}2-\frac{1}6 = \frac{1}3$. 

</div>